\documentclass[12pt]{article}
 
\usepackage[margin=1in]{geometry} 
\usepackage{amsmath,amsthm,amssymb}
 
\newcommand{\N}{\mathbb{N}}
\newcommand{\Z}{\mathbb{Z}}
\newcommand{\Q}{\mathbb{Q}}
\newcommand{\R}{\mathbb{R}}
\newcommand{\C}{\mathbb{C}}
 
\newenvironment{theorem}[2][Theorem]{\begin{trivlist}
\item[\hskip \labelsep {\bfseries #1}\hskip \labelsep {\bfseries #2.}]}{\end{trivlist}}
\newenvironment{lemma}[2][Lemma]{\begin{trivlist}
\item[\hskip \labelsep {\bfseries #1}\hskip \labelsep {\bfseries #2.}]}{\end{trivlist}}
\newenvironment{exercise}[2][Exercise]{\begin{trivlist}
\item[\hskip \labelsep {\bfseries #1}\hskip \labelsep {\bfseries #2.}]}{\end{trivlist}}
\newenvironment{problem}[2][Problem]{\begin{trivlist}
\item[\hskip \labelsep {\bfseries #1}\hskip \labelsep {\bfseries #2.}]}{\end{trivlist}}
\newenvironment{question}[2][Question]{\begin{trivlist}
\item[\hskip \labelsep {\bfseries #1}\hskip \labelsep {\bfseries #2.}]}{\end{trivlist}}
\newenvironment{corollary}[2][Corollary]{\begin{trivlist}
\item[\hskip \labelsep {\bfseries #1}\hskip \labelsep {\bfseries #2.}]}{\end{trivlist}}

%\begin{align*}
%\end{align*}
 
\begin{document}
 
\title{Homework 4} 
\author{J.E. Paguyo \\ MAT 185A} 
\maketitle
 
\begin{exercise}{1} Let $f: G \to \C$ be a continuous function on an open set $G \subset \C$ and let $\gamma : [a,b] \to \C$ be a piecewise smooth curve in $G$. 
\end{exercise}
 
\noindent a) Find a counterexample demonstrating that the inequality 
\begin{align*}
\left| \int_{\gamma} f(z) \, dz \right| \leq \int_{\gamma} |f(z)| \, dz
\end{align*}
no longer makes sense for integrals along a curve $\gamma$. \\ \\
{\em Proof}. 
$\hfill \qed$ \\

\noindent b) Show that 
\begin{align*}
\left| \int_{\gamma} f(z) \right| \leq \int_{\gamma} |f(z)| \, |dz|
\end{align*}
where the latter is defined by 
\begin{align*}
\int_{\gamma} |f(z)| \, |dz| = \int_a^b |f(\gamma (t))||\gamma'(t)| \, dt 
\end{align*} \\ \\ 
{\em Proof}.
$\hfill \qed$ \\

\begin{exercise}{2} Deduce from Exercise 1 that 
\begin{align*}
\left| \int_{\gamma} f \right| \leq Ml(\gamma)
\end{align*}
where $M \geq 0$ is a real constant such that $|f(z)| \leq M$ for all points $z$ on $\gamma$ and 
\begin{align*}
l(y) = \int_a^b |\gamma'(t)| \, dt = \int_a^b \sqrt{x'(t)^2 + y'(t)^2} \, dt
\end{align*}
is the length of the curve. 
\end{exercise}
 
\begin{proof} We have that 
\begin{align*}
\left| \int_{\gamma} f(z) \right| &= \left| \int_a^b f(\gamma(t)) \gamma'(t) \, dt \right| \leq \int_a^b |f(\gamma(t))||\gamma'(t)| \, dt = \int_a^b M|\gamma'(t)| \, dt \\
&= M\int_a^b |\gamma'(t)| \, dt = Ml(\gamma)
\end{align*}
Where the inequality is from Exercise 1
\end{proof}

\begin{exercise}{3} Let $\gamma$ be the arc of the circle $|z| = 2$ in the first quadrant $(x,y>0)$. Establish the inequality
\begin{align*}
\left| \int_{\gamma} \frac{dz}{1 + z^2} \right| \leq \frac{\pi}{3}
\end{align*}
without performing the integral explicitly. 
\end{exercise}
 
\begin{proof}

\end{proof}

\begin{exercise}{4} Compute $\int_{\gamma} f(z) \, dz$ for the following 
\end{exercise}
 
\noindent a) $f(z) = -y^2 + x^2 - 2ixy$ and $\gamma$ the straight line from $0$ to $-1-i$. \\ \\ 
{\em Proof}.
$\hfill \qed$ \\

\noindent b) $f(z) = (2+z)/z$ and $\gamma$ the semi-circle $z = e^{i\theta}$, $0 \leq \theta \leq \pi$. \\ \\
{\em Proof}.
$\hfill \qed$ \\

\noindent c) $f(z) = 1/z$ and $\gamma$ any path in the right half plane $\text{Re}(z) \geq 0$ beginning at $-i$, ending at $i$, avoiding the origin. \\ \\ 
{\em Proof}.
$\hfill \qed$ 

\begin{exercise}{5} Let $f,g$ be continuous functions, $c_1,c_2$ complex constants, and $\gamma,\gamma_1,\gamma_2$ piecewise smooth curves. Show that
\end{exercise}
 
\noindent a) $\int_{\gamma} (c_1f+c_2g) = c_1\int_{\gamma} f + c_2\int_{\gamma} g$ \\ \\
{\em Proof}.
\begin{align*}
\int_{\gamma} (c_1f+c_2g) &= \int_a^b (c_1f(\gamma(t)) + c_2g(\gamma(t))) \gamma'(t) \, dt = \int_a^b (c_1f(\gamma(t)) \gamma'(t) + c_2g(\gamma(t)) \gamma'(t) ) \, dt \\ 
&= \int_a^b c_1f(\gamma(t)) \gamma'(t) \, dt + \int_a^b c_2g(\gamma(t)) \gamma'(t) \, dt \\ &= c_1 \int_a^b f(\gamma(t)) \gamma'(t) \, dt + c_2 \int_a^b g(\gamma(t)) \gamma'(t) \, dt \\
&= c_1\int_{\gamma} f + c_2\int_{\gamma} g
\end{align*}
$\hfill \qed$ \\

\noindent b) $\int_{-\gamma} f = -\int_{\gamma} f$ \\ \\
{\em Proof}.
\begin{align*}
\int_{-\gamma} f = \int_a^b f(\gamma(t)) (-\gamma'(t)) \, dt = - \int_a^b f(\gamma(t)) \gamma'(t) \, dt = -\int_{\gamma} f
\end{align*}
$\hfill \qed$ \\

\noindent c) $\int_{\gamma_1 + \gamma_2} f = \int_{\gamma_1} f + \int_{\gamma_2} f$ \\ \\ 
{\em Proof}.
$\hfill \qed$ 

\end{document}